ArkLib.lean
@@ -83,10 +83,11 @@ import ArkLib.Data.Probability.Notation
 import ArkLib.Interaction.Basic.Append
 import ArkLib.Interaction.Basic.BundledMonad
 import ArkLib.Interaction.Basic.Chain
+import ArkLib.Interaction.Basic.Spec
+import ArkLib.Interaction.Basic.Node
 import ArkLib.Interaction.Basic.Decoration
 import ArkLib.Interaction.Basic.MonadDecoration
 import ArkLib.Interaction.Basic.Replicate
-import ArkLib.Interaction.Basic.Spec
 import ArkLib.Interaction.Basic.Shape
 import ArkLib.Interaction.Basic.Interaction
 import ArkLib.Interaction.Basic.StateChain
